
### Trigonometrical identities:

Summation of angles:

$$ \cos(\frac \pi 2 +\alpha)=\sin(\alpha) $$

$$ \sin(\alpha - \frac \pi 2)=\cos(\alpha) $$

$$ \sin(\alpha+\beta)=\sin(\alpha)\cos(\beta) + \sin(\beta)\cos(\alpha) $$

$$ \sin(\alpha-\beta)=\sin(\alpha)\cos(\beta) - \sin(\beta)\cos(\alpha) $$

$$ \cos(\alpha+\beta)=\cos(\alpha)\cos(\beta) -\sin(\beta)\sin(\alpha) $$

$$ \cos(\alpha-\beta)=\cos(\alpha)\cos(\beta) + \sin(\beta)\sin(\alpha) $$

$$ \tan(\alpha+\beta)=\frac{\tan(\alpha)+\tan(\beta)}{1-\tan(\alpha)\tan(\beta)} $$

$$ \tan(\alpha-\beta)=\frac{\tan(\alpha)-\tan(\beta)}{1+\tan(\alpha)\tan(\beta)} $$

Duplication Formula:

$$ \sin(2\alpha)=2\sin(\alpha)\cos(\alpha) $$

$$ \cos(2\alpha)=\cos^2(\alpha)-\sin^2(\alpha) $$

$$ \tan(2\alpha)=\frac{2\tan(\alpha)}{1-\tan^2(\alpha)} $$

(We can find those formula by replacing beta by alpha in the summation formula).

And because

$$ \cos^2(\alpha)+\sin^2(\alpha)=1 $$

We have:

$$ \cos(2\alpha)=2\cos^2(\alpha)-1=1-2\sin^2(\alpha) $$

And so finally, Carnot formula:

$$ \cos^2(\alpha)=\frac{1+\cos(2\alpha)}{2} $$

$$ \sin^2(\alpha)=\frac{1-\cos(2\alpha)}{2} $$